# Reverse Substrings Between Each Pair of Parentheses

## Problem Description

You are given a string `s` that consists of lowercase English letters and brackets. The task is to reverse the strings in each pair of matching parentheses, starting from the innermost one. The result should not contain any brackets.

### Examples

#### Example 1

**Input:** `s = "(abcd)"`

**Output:** `dcba`

#### Example 2

**Input:** `s = "(u(love)i)"`

**Output:** `iloveu`

**Explanation:** The substring "love" is reversed first, then the whole string is reversed.

#### Example 3

**Input:** `s = "(ed(et(oc))el)"`

**Output:** `leetcode`

**Explanation:** First, the substring "oc" is reversed, then "etco", and finally, the whole string.

## Solution

The solution involves using a stack to keep track of the indices of the opening brackets. When a closing bracket is encountered, the corresponding opening bracket is popped from the stack, and the substring between these brackets is reversed. This process is repeated from the innermost pair of parentheses to the outermost.

### Algorithm

1. Initialize a stack to keep track of the indices of the opening brackets.
2. Iterate through the string:
    - When an opening bracket is encountered, push its index onto the stack.
    - When a closing bracket is encountered, pop the index of the corresponding opening bracket from the stack and reverse the substring between these indices.
3. Use a dictionary to store the pairs of indices of matching brackets.
4. Use a result list to construct the final output by iterating through the string and reversing the necessary substrings.

### Solution Code

```python
class Solution:
    def reverseParentheses(self, s: str) -> str:
        result = []
        pair = {}
        stack = []

        for i, c in enumerate(s):
            if c == "(":
                stack.append(i)
            elif c == ")":
                j = stack.pop()
                pair[i] = j
                pair[j] = i
        
        i = 0
        d = 1

        while i < len(s):
            if s[i] in '()':
                i = pair[i]
                d = -d
            else:
                result.append(s[i])
            i += d
        
        return ''.join(result)
